Add correctness conditions for gcm_init_v8

Proofs/AES-GCM/GCMInitV8Sym.lean
@@ -6,21 +6,78 @@ Author(s): Yan Peng
 import Proofs.«AES-GCM».GCMInitV8Pre
 import Tactics.Sym
 import Tactics.Aggregate
+import Specs.GCMV8
 
 namespace GCMInitV8Program
 
+abbrev H_addr (s : ArmState) : BitVec 64 := r (StateField.GPR 1#5) s
+abbrev Htable_addr (s : ArmState) : BitVec 64 := r (StateField.GPR 0#5) s
+
+set_option debug.byAsSorry true in
 set_option maxRecDepth 1000000 in
--- set_option diagnostics true in
 set_option profiler true in
 theorem gcm_init_v8_program_run_152 (s0 sf : ArmState)
     (h_s0_program : s0.program = gcm_init_v8_program)
     (h_s0_err : read_err s0 = .None)
     (h_s0_pc : read_pc s0 = gcm_init_v8_program.min)
     (h_s0_sp_aligned : CheckSPAlignment s0)
-    (h_run : sf = run gcm_init_v8_program.length s0) :
-    read_err sf = .None := by
+    (h_run : sf = run gcm_init_v8_program.length s0)
+    (h_mem : Memory.Region.pairwiseSeparate
+      [ ⟨(H_addr s0), 128⟩,
+        ⟨(Htable_addr s0), 2048⟩ ])
+    : read_err sf = .None := by
   simp (config := {ground := true}) only at h_s0_pc
   -- ^^ Still needed, because `gcm_init_v8_program.min` is somehow
   --    unable to be reflected
   sym_n 152
   done
+
+-- TODO: this function is from Tests.Common
+-- need to put it in a better place
+def revflat (x : List (BitVec n)) : BitVec (n * x.length) :=
+  have h : n * x.reverse.length = n * x.length := by simp only [List.length_reverse]
+  BitVec.cast h $ BitVec.flatten (List.reverse x)
+
+
+set_option maxRecDepth 1000000 in
+set_option maxHeartbeats 2000000 in
+set_option profiler true in
+theorem gcm_init_v8_program_correct (s0 sf : ArmState)
+    (h_s0_program : s0.program = gcm_init_v8_program)
+    (h_s0_err : read_err s0 = .None)
+    (h_s0_pc : read_pc s0 = gcm_init_v8_program.min)
+    (h_s0_sp_aligned : CheckSPAlignment s0)
+    (h_run : sf = run gcm_init_v8_program.length s0)
+    (h_mem : Memory.Region.pairwiseSeparate
+      [ ⟨(H_addr s0), 128⟩,
+        ⟨(Htable_addr s0), 2048⟩ ])
+    : -- effects
+      -- no instruction decoding error
+      read_err sf = .None
+      -- program is unchanged
+    ∧ sf.program = gcm_init_v8_program
+      -- SP is still aligned
+    ∧ CheckSPAlignment s0
+      -- PC is updated
+    ∧ read_pc sf = 0x79f5ec#64
+      -- First 12 elemets in Htable is correct
+    ∧ read_mem_bytes 192 (Htable_addr sf) sf
+      = revflat (GCMV8.GCMInitV8 (read_mem_bytes 16 (H_addr s0) s0))
+    -- non-effects
+    -- State values that shouldn't change do not change
+    -- TODO: figure out all registers that are used ...
+    ∧ (∀ (f : StateField), ¬ (f = StateField.PC) ∧
+                           ¬ (f = (StateField.GPR 29#5)) →
+        r f sf = r f s0)
+    -- Memory safety: memory location that should not change did
+    -- not change
+    -- The addr exclude output region Htable
+    ∧ (∀ (n : Nat) (addr : BitVec 64) (h: addr < (Htable_addr sf) ∧ addr >= (Htable_addr sf) + 128*12),
+        read_mem_bytes n addr sf = read_mem_bytes n addr s0)
+    := by
+  simp (config := {ground := true}) only at h_s0_pc
+  -- ^^ Still needed, because `gcm_init_v8_program.min` is somehow
+  --    unable to be reflected
+  sym_n 152
+  sym_aggregate
+  sorry
